compiler/src/compiler/UseImmediate.v
@@ -25,40 +25,131 @@ Section WithArguments.
        morphism (word.ring_morph (word := word)),
         constants [word_cst]).
 
-  Local Hint Constructors exec: core.
-  Local Notation exec := (exec isRegStr).
+  Local Notation exec := (exec PreSpill isRegStr).
+
+  Open Scope MetricH_scope.
+
+  Ltac tandem H := (
+    repeat match goal with
+           | |- exists _, _ => let x := fresh in destruct H as (x&?); exists x
+           | |- _ /\ _ => destruct H as (?&H); split; try eassumption
+           | _ => let x := fresh in intro x; specialize (H x)
+           end
+  ).
+
+  Ltac finish := (
+    simpl;
+    intros *;
+    repeat match goal with
+           | |- (exists _, _ /\ _) -> _ => intros (?&?&?)
+           | |- _ /\ _ => split; eauto
+           | |- exists _, _ => eexists
+           end;
+    repeat match goal with
+           | H : _ <= _ |- _ => revert H
+           end;
+    clear;
+    unfold exec.cost_SInteract, exec.cost_SCall_internal,
+    exec.cost_SCall_external, exec.cost_SLoad, exec.cost_SStore,
+    exec.cost_SInlinetable, exec.cost_SStackalloc, exec.cost_SLit,
+    exec.cost_SOp, exec.cost_SSet, exec.cost_SIf, exec.cost_SLoop_true,
+    exec.cost_SLoop_false;
+    repeat match goal with
+           | x : operand |- _ => destr x
+           | x : bcond _ |- _ => destr x
+           | |- context[isRegStr ?x] => destr (isRegStr x)
+           end;
+    try solve_MetricLog
+  ).
+
+  (* TODO these two lemmas are somewhat slow *)
+  Lemma op_cost_y : forall x0 y v0 mcH' mc v mcL lit,
+    exec.cost_SOp isRegStr x0 y (Var v0) EmptyMetricLog - EmptyMetricLog <=
+      mcH' - exec.cost_SLit isRegStr lit mc ->
+    exec.cost_SOp isRegStr x0 y (Const v) (exec.cost_SLit isRegStr lit mcL) - mcL <=
+      mcH' - mc.
+  Proof. finish. Qed.
+
+  Lemma op_cost_v0 : forall x0 y v0 mcH' mc v mcL lit,
+    exec.cost_SOp isRegStr x0 y (Var v0) EmptyMetricLog - EmptyMetricLog <=
+      mcH' - exec.cost_SLit isRegStr lit mc ->
+    exec.cost_SOp isRegStr x0 v0 (Const v) (exec.cost_SLit isRegStr lit mcL) - mcL <=
+      mcH' - mc.
+  Proof. finish. Qed.
 
   Lemma useImmediate_correct_aux:
     forall eH eL,
        (useimmediate_functions is5BitImmediate is12BitImmediate) eH = Success eL ->
        forall sH t m mcH lH post,
        exec eH sH t m lH mcH post ->
-       exec eL (useImmediate is5BitImmediate is12BitImmediate sH) t m lH mcH post.
+       forall mcL,
+       exec eL (useImmediate is5BitImmediate is12BitImmediate sH) t m lH mcL
+       (fun t' m' l' mcL' => exists mcH', metricsLeq (mcL' - mcL) (mcH' - mcH) /\ post t' m' l' mcH').
   Proof.
-    induction 2.
-    (* most cases stay the same *)
-    all: try solve [simpl; eauto].
+    induction 2; try solve [
+      simpl; econstructor; eauto;
+      tandem H3;
+      finish
+    ].
 
-    (* SCall *)
-    { simpl.
-      eapply @exec.call; try eassumption.
-      assert (exists v2, (useimmediate_function is5BitImmediate is12BitImmediate) (params, rets, fbody) = Success v2 /\ map.get eL fname = Some v2).
-      { eapply map.try_map_values_fw.
-        - simpl in H; eapply H.
-        - eassumption.
-      }
-      destruct H5. destruct H5. simpl in H5. inversion H5. fwd.
-      eassumption.
-    }
+    - (* SCall *)
+      simpl; econstructor; eauto.
+      { unfold useimmediate_functions in H.
+        destruct (map.try_map_values_fw _ _ _ H _ _ H0) as (?&[=Huseimm]&Hmap).
+        rewrite <- Huseimm in Hmap.
+        exact Hmap. }
+      cbv beta.
+      intros * (?&?&Houtcome).
+      destruct (H4 _ _ _ _ Houtcome) as (retvs&l'&Hpost).
+      exists retvs, l'.
+      tandem Hpost.
+      finish.
 
-    (* SSeq *)
-    { simpl.
-      repeat (match goal with
-              | |- context[match ?x with _ => _ end] => destr x
-              | |- context[if ?x then _ else _ ] => destr x
-              end;
-              try solve [eapply @exec.seq; eassumption]);
-        simpl in *.
+    - (* SStackalloc *)
+      simpl; econstructor; eauto.
+      tandem H2.
+      eapply exec.weaken; [eauto|].
+      simpl; intros * (?&?&?&?&?&?&?).
+      finish.
+
+    - (* SIf true *)
+      simpl; econstructor; eauto.
+      eapply exec.weaken; [eauto|].
+      finish.
+
+    - (* SIf false *)
+      simpl; intro; eapply exec.if_false; eauto.
+      eapply exec.weaken; [eauto|].
+      finish.
+
+    - (* SLoop *)
+      simpl; econstructor; eauto; simpl.
+      { intros * (?&?&?); eauto. }
+      { intros * (?&?&?) **. finish. }
+      { intros * (?&?&?) **.
+        eapply exec.weaken; [eauto|].
+        simpl; intros * (?&?&?).
+        instantiate (1 := fun t m l MC1 => exists MC2, MC1 - mcL <= MC2 - mc /\ mid2 t m l MC2).
+        finish. }
+      { intros * (?&?&?).
+        eapply exec.weaken; [eauto|].
+        finish. }
+
+    - (* SSeq *)
+      simpl. intro.
+
+      repeat (
+        match goal with
+        | |- context[match ?x with _ => _ end] => destr x
+        | |- context[if ?x then _ else _ ] => destr x
+        end;
+        try solve [
+          eapply @exec.seq; eauto; simpl;
+          intros * (?&?&?);
+          eapply @exec.weaken; [eauto|];
+          finish
+        ]
+      ).
 
       all: eapply @exec.seq_cps; eapply @exec.lit.
 
@@ -71,10 +162,10 @@ Section WithArguments.
 
       all: match goal with
            | H: ?mid _ _ _ _,
-               H0: forall t m l mc,
-                 ?mid t m l mc -> exec ?eL _ _ _ _ _ ?post
-                 |- exec ?eL _ _ _ _ _ ?post
-             => apply H0 in H; inversion H
+             H0: forall t m l mc,
+                 ?mid t m l mc -> forall mcL, exec ?eL _ _ _ _ mcL _
+                 |- exec ?eL _ _ _ _ _ _
+             => specialize (H0 _ _ _ _ H EmptyMetricLog); inversion H0
            end.
 
       all: simpl in *;
@@ -83,14 +174,17 @@ Section WithArguments.
           => rewrite map.get_put_same in H; fwd
         end.
 
-      all: eapply @exec.op; simpl in *; [ eassumption |  reflexivity | try eassumption ].
+      all: eapply @exec.op; simpl in *; [ eassumption | reflexivity | ].
 
-      all: admit.
-      (*{ rewrite word.add_comm. assumption. }*)
-      (*{ replace (word.add y' (word.of_Z (- v)))  with  (word.sub  y' (word.of_Z v)) by ring. assumption. }*)
-      (*{ rewrite word.and_comm. assumption. }*)
-      (*{ rewrite word.or_comm. assumption. }*)
-      (*{ rewrite word.xor_comm. assumption. }*)
-    }
-  Admitted.
+      all: exists mcH'; split; [solve [eapply op_cost_y; eauto | eapply op_cost_v0; eauto]|eauto].
+
+      + rewrite word.add_comm. assumption.
+      + replace (word.add y' (word.of_Z (-v))) with (word.sub y' (word.of_Z v)) by ring. assumption.
+      + rewrite word.and_comm. assumption.
+      + rewrite word.or_comm. assumption.
+      + rewrite word.xor_comm. assumption.
+
+  (* this is slightly slow also *)
+  Qed.
+
 End WithArguments.
